proof/refine/ARM_HYP/Interrupt_R.thy
@@ -1185,7 +1185,6 @@ lemma vgicMaintenance_invs'[wp]:
              apply (clarsimp simp: invs'_def valid_state'_def valid_idle'_def obj_at'_def idle_tcb'_def)
             apply wps
             apply (wpsimp simp: if_apply_def2 wp: hoare_vcg_const_imp_lift hoare_drop_imps
-hoare_vcg_ex_lift hoare_vcg_conj_lift
                    | wps)+
   apply (clarsimp cong: conj_cong imp_cong split: if_split)
   apply (strengthen st_tcb_ex_cap''[where P=active'])
